Upgrade to 9.2

src/FrameStack/LabeledTermination.v
@@ -20,163 +20,160 @@ match a with
 end.
 
 (** A more practical way to define termination in k steps *)
-Set Warnings "-closed-notation-not-level-0".
-(* The following notation does not work with level 0 *)
-Reserved Notation "| fs , e | l – k ↓" (at level 80).
-Set Warnings "+closed-notation-not-level-0".
+Reserved Notation "⟨ fs , e ⟩ l – k ↓" (at level 0).
 Inductive terminates_in_k : FrameStack -> Redex -> SideEffectList -> nat -> Prop :=
 
 (** Cooling: single value *)
 | cool_value_l v xs l k :
-  | xs, RValSeq [v] | l – k ↓
+  ⟨ xs, RValSeq [v] ⟩ l – k ↓
 ->
-  | xs, ˝v | l – S k ↓
+  ⟨ xs, ˝v ⟩ l – S k ↓
 
 (************************************************)
 (* heating should be separate for all complex expressions (to be
    syntax-driven).
    Only the intermediate and last steps can be extracted: *)
 | step_params xs ident (el : list Exp) (vl : list Val) (v : Val) (e : Exp) l k:
-  | FParams ident (vl ++ [v]) el :: xs, e | l – k ↓
+  ⟨ FParams ident (vl ++ [v]) el :: xs, e ⟩ l – k ↓
 ->
-  | FParams ident vl (e :: el) :: xs, RValSeq [v] | l – S k ↓
+  ⟨ FParams ident vl (e :: el) :: xs, RValSeq [v] ⟩ l – S k ↓
 
 (* technical rule to avoid duplication for 0 subexpressions : *)
 | step_params_0 xs ident e (el : list Exp) vl l k:
   ident <> IMap ->
-  |FParams ident vl el :: xs, RExp e| l – k ↓
+  ⟨FParams ident vl el :: xs, RExp e⟩ l – k ↓
 ->
-  |FParams ident vl (e::el) ::xs, RBox| l – S k ↓
+  ⟨FParams ident vl (e::el) ::xs, RBox⟩ l – S k ↓
 
 (* 0 subexpression in complex expressions: *)
 | cool_params_0_l xs ident (vl : list Val) (res : Redex) (l: option SideEffect) ls k: 
   ident <> IMap ->
   Some (res, l) = create_result ident vl -> (* TODO side effects *)
-  |xs, res| ls – k ↓
+  ⟨xs, res⟩ ls – k ↓
 ->
-  |FParams ident vl [] ::xs, RBox| (option_cons l ls) – S k ↓
+  ⟨FParams ident vl [] ::xs, RBox⟩ (option_cons l ls) – S k ↓
 
 | cool_params xs ident (vl : list Val) (v : Val) (res : Redex) (l : option SideEffect) ls k:
   Some (res, l) = create_result ident (vl ++ [v]) -> (* TODO side effects *)
-  |xs, res| ls – k ↓
+  ⟨xs, res⟩ ls – k ↓
 ->
-  |FParams ident vl [] :: xs, RValSeq [v]| (option_cons l ls) – S k ↓
+  ⟨FParams ident vl [] :: xs, RValSeq [v]⟩ (option_cons l ls) – S k ↓
 
 (************************************************)
 (* Heating constructs with list subexpressions: *)
 | heat_values (el : list Exp) (xs : list Frame) l k:
-  | (FParams IValues [] el)::xs, RBox | l – k ↓
+  ⟨ (FParams IValues [] el)::xs, RBox ⟩ l – k ↓
 ->
-  | xs, EValues el | l – S k ↓
+  ⟨ xs, EValues el ⟩ l – S k ↓
 
 | heat_tuple (el : list Exp) (xs : list Frame) l k:
-  | (FParams ITuple [] el)::xs, RBox | l – k ↓ 
+  ⟨ (FParams ITuple [] el)::xs, RBox ⟩ l – k ↓ 
 ->
-  | xs, ETuple el | l – S k ↓
+  ⟨ xs, ETuple el ⟩ l – S k ↓
 
 (* This is handled separately, to satisfy the invariant in FCLOSED for maps *)
 | heat_map_0 (xs : list Frame) l k:
-  | xs, RValSeq [VMap []] | l – k ↓ 
+  ⟨ xs, RValSeq [VMap []] ⟩ l – k ↓ 
 ->
-  | xs, EMap [] | l – S k ↓
+  ⟨ xs, EMap [] ⟩ l – S k ↓
 
 | heat_map (e1 e2 : Exp) (el : list (Exp * Exp)) (xs : list Frame) l k:
-  | (FParams IMap [] (e2 :: flatten_list el))::xs, e1 | l – k ↓ 
+  ⟨ (FParams IMap [] (e2 :: flatten_list el))::xs, e1 ⟩ l – k ↓ 
 ->
-  | xs, EMap ((e1, e2) :: el) | l – S k ↓
+  ⟨ xs, EMap ((e1, e2) :: el) ⟩ l – S k ↓
 
 | heat_call_mod (el : list Exp) (xs : list Frame) (m f : Exp) l k :
-  | FCallMod f el :: xs, m | l – k ↓
+  ⟨ FCallMod f el :: xs, m ⟩ l – k ↓
 ->
-  | xs, ECall m f el | l – S k ↓
+  ⟨ xs, ECall m f el ⟩ l – S k ↓
 
 | heat_call_fun (el : list Exp) (xs : list Frame) (v : Val) (f : Exp) l k :
-  | FCallFun v el :: xs, f | l – k ↓
+  ⟨ FCallFun v el :: xs, f ⟩ l – k ↓
 ->
-  | FCallMod f el :: xs, RValSeq [v] | l – S k ↓
+  ⟨ FCallMod f el :: xs, RValSeq [v] ⟩ l – S k ↓
 
 | heat_call_params (el : list Exp) (xs : list Frame) (m f : Val) l k:
-  | (FParams (ICall m f) [] el)::xs, RBox | l – k ↓
+  ⟨ (FParams (ICall m f) [] el)::xs, RBox ⟩ l – k ↓
 ->
-  | FCallFun m el :: xs, RValSeq [f] | l – S k ↓
+  ⟨ FCallFun m el :: xs, RValSeq [f] ⟩ l – S k ↓
 
 | heat_primop (el : list Exp) (xs : list Frame) f l k:
-  | (FParams (IPrimOp f) [] el)::xs, RBox | l – k ↓ 
+  ⟨ (FParams (IPrimOp f) [] el)::xs, RBox ⟩ l – k ↓ 
 ->
-  | xs, EPrimOp f el | l – S k ↓
+  ⟨ xs, EPrimOp f el ⟩ l – S k ↓
 
 | heat_app2 (el : list Exp) (xs : list Frame) (v : Val) l k:
-  | (FParams (IApp v) [] el)::xs, RBox | l – k ↓ 
+  ⟨ (FParams (IApp v) [] el)::xs, RBox ⟩ l – k ↓ 
 ->
-  | FApp1 el :: xs, RValSeq [v] | l – S k ↓
+  ⟨ FApp1 el :: xs, RValSeq [v] ⟩ l – S k ↓
 
 (************************************************)
 (**  App *)
 | heat_app xs e l ls k:
-  |FApp1 l :: xs, RExp e| ls – k ↓ 
+  ⟨FApp1 l :: xs, RExp e⟩ ls – k ↓ 
 ->
-  |xs, EApp e l| ls – S k ↓
+  ⟨xs, EApp e l⟩ ls – S k ↓
 (**  List *)
 (**  Cooling *)
 
 | cool_cons_1 (hd : Exp) (tl : Val) xs l k :
-  | (FCons2 tl)::xs, RExp hd | l – k ↓ 
+  ⟨ (FCons2 tl)::xs, RExp hd ⟩ l – k ↓ 
 ->
-  | (FCons1 hd)::xs, RValSeq [tl] | l – S k ↓
+  ⟨ (FCons1 hd)::xs, RValSeq [tl] ⟩ l – S k ↓
 
 | cool_cons_2 (hd tl : Val) xs l k:
-  | xs, RValSeq [VCons hd tl] | l – k ↓ 
+  ⟨ xs, RValSeq [VCons hd tl] ⟩ l – k ↓ 
 ->
-  | (FCons2 tl)::xs, RValSeq [hd] | l – S k ↓
+  ⟨ (FCons2 tl)::xs, RValSeq [hd] ⟩ l – S k ↓
 
 (**  Heating *)
 | heat_cons (hd tl : Exp) xs l k:
-  | (FCons1 hd)::xs, RExp tl | l – k ↓ 
+  ⟨ (FCons1 hd)::xs, RExp tl ⟩ l – k ↓ 
 ->
-  | xs, ECons hd tl | l – S k ↓
+  ⟨ xs, ECons hd tl ⟩ l – S k ↓
 
 (**  Let *)
 (**  Cooling *)
 | cool_let l e2 vs xs ls k:
   length vs = l ->
-  | xs, RExp (e2.[ list_subst vs idsubst ]) | ls – k ↓ 
+  ⟨ xs, RExp (e2.[ list_subst vs idsubst ]) ⟩ ls – k ↓ 
 ->
-  | (FLet l e2)::xs, RValSeq vs | ls – S k ↓
+  ⟨ (FLet l e2)::xs, RValSeq vs ⟩ ls – S k ↓
 
 (**  Heating *)
 | heat_let l e1 e2 xs ls k:
-  | (FLet l e2)::xs, RExp e1 | ls – k ↓ 
+  ⟨ (FLet l e2)::xs, RExp e1 ⟩ ls – k ↓ 
 ->
-  | xs, ELet l e1 e2 | ls – S k ↓
+  ⟨ xs, ELet l e1 e2 ⟩ ls – S k ↓
 
 (**  Seq *)
 (**  Cooling *)
 | cool_seq e2 v xs l k:
-  | xs, RExp e2 | l – k ↓ 
+  ⟨ xs, RExp e2 ⟩ l – k ↓ 
 ->
-  | (FSeq e2)::xs, RValSeq [v] | l – S k ↓
+  ⟨ (FSeq e2)::xs, RValSeq [v] ⟩ l – S k ↓
 (**  Heating *)
 | heat_seq e1 e2 xs l k:
-  | (FSeq e2)::xs, RExp e1 | l – k ↓ 
+  ⟨ (FSeq e2)::xs, RExp e1 ⟩ l – k ↓ 
 ->
-  | xs, ESeq e1 e2 | l – S k ↓
+  ⟨ xs, ESeq e1 e2 ⟩ l – S k ↓
 
 
 (**  Fun *)
 (**  Cooling *)
 | cool_fun e vl xs l k:
-  | xs, RValSeq [ VClos [] 0 vl e ] | l – k ↓ 
+  ⟨ xs, RValSeq [ VClos [] 0 vl e ] ⟩ l – k ↓ 
 ->
-  | xs, EFun vl e | l – S k ↓
+  ⟨ xs, EFun vl e ⟩ l – S k ↓
   (* TODO : id <> 0 usually *)
 
 
 (**  Case *)
 (**  Heating *)
 | heat_case e l xs ls k:
-  | (FCase1 l)::xs, RExp e | ls – k ↓ 
+  ⟨ (FCase1 l)::xs, RExp e ⟩ ls – k ↓ 
 ->
-  | xs, ECase e l | ls – S k ↓
+  ⟨ xs, ECase e l ⟩ ls – S k ↓
 
 (**  Cooling *)
 (* reduction started or it is already ongoing, the first pattern matched,
@@ -184,36 +181,36 @@ Inductive terminates_in_k : FrameStack -> Redex -> SideEffectList -> nat -> Prop
    matching is stored in the frame) *)
 | step_case_match lp e1 e2 l vs vs' xs ls k:
   match_pattern_list lp vs = Some vs' ->
-  | (FCase2 vs e2.[list_subst vs' idsubst] l)::xs, RExp (e1.[list_subst vs' idsubst]) | ls – k ↓
+  ⟨ (FCase2 vs e2.[list_subst vs' idsubst] l)::xs, RExp (e1.[list_subst vs' idsubst]) ⟩ ls – k ↓
 ->
-  | (FCase1 ((lp,e1,e2)::l))::xs, RValSeq vs | ls – S k ↓
+  ⟨ (FCase1 ((lp,e1,e2)::l))::xs, RValSeq vs ⟩ ls – S k ↓
 (* reduction started or it is already ongoing, the first pattern doesn't 
    match, so we check the next pattern *)
 | step_case_not_match lp e1 e2 l vs xs ls k:
   match_pattern_list lp vs = None ->
-  | (FCase1 l)::xs, RValSeq vs | ls – k ↓ 
+  ⟨ (FCase1 l)::xs, RValSeq vs ⟩ ls – k ↓ 
 ->
-  | (FCase1 ((lp,e1,e2)::l))::xs, RValSeq vs | ls – S k ↓
+  ⟨ (FCase1 ((lp,e1,e2)::l))::xs, RValSeq vs ⟩ ls – S k ↓
 
 (* reduction is ongoing, the pattern matched, and the guard is true, thus 
    the reduction continues inside the given clause *)
 | step_case_true_l vs e' l xs ls k:
-  | xs, RExp e' | ls – k ↓ 
+  ⟨ xs, RExp e' ⟩ ls – k ↓ 
 ->
-  | (FCase2 vs e' l)::xs, RValSeq [ VLit (Atom "true") ] | ls – S k ↓
+  ⟨ (FCase2 vs e' l)::xs, RValSeq [ VLit (Atom "true") ] ⟩ ls – S k ↓
 
 (* reduction is ongoing, the pattern matched, and the guard is false, thus
    we check the next pattern. *)
 | step_case_false_l vs e' l xs k ls:
-  | (FCase1 l)::xs, RValSeq vs | ls – k ↓ 
+  ⟨ (FCase1 l)::xs, RValSeq vs ⟩ ls – k ↓ 
 ->
-  | (FCase2 vs e' l)::xs, RValSeq [ VLit (Atom "false") ] | ls – S k ↓
+  ⟨ (FCase2 vs e' l)::xs, RValSeq [ VLit (Atom "false") ] ⟩ ls – S k ↓
 
 (** Exceptions *)
 | cool_case_empty vs xs l k:
-  | xs, RExc if_clause | l – k ↓ 
+  ⟨ xs, RExc if_clause ⟩ l – k ↓ 
 ->
-  | (FCase1 [])::xs, RValSeq vs | l – S k ↓
+  ⟨ (FCase1 [])::xs, RValSeq vs ⟩ l – S k ↓
 
 (**  LetRec *)
 (**  Cooling *)
@@ -221,71 +218,71 @@ Inductive terminates_in_k : FrameStack -> Redex -> SideEffectList -> nat -> Prop
 | heat_letrec l e lc xs ls k:
   convert_to_closlist (map (fun '(x,y) => (0,x,y)) l) = lc ->
   (* TODO: for now the funids are 0 coded in *)
-  | xs, RExp e.[list_subst lc idsubst] | ls – k ↓ 
+  ⟨ xs, RExp e.[list_subst lc idsubst] ⟩ ls – k ↓ 
 ->
-  | xs, ELetRec l e | ls – S k ↓
+  ⟨ xs, ELetRec l e ⟩ ls – S k ↓
 
 
 (**  Try *)
 (**  Cooling *)
 | cool_try_ok vl1 e2 vl2 e3 vs xs l k:
   vl1 = length vs ->
-  | xs, RExp e2.[ list_subst vs idsubst ] | l – k ↓ 
+  ⟨ xs, RExp e2.[ list_subst vs idsubst ] ⟩ l – k ↓ 
 ->
-  | (FTry vl1 e2 vl2 e3)::xs, RValSeq vs | l – S k ↓
+  ⟨ (FTry vl1 e2 vl2 e3)::xs, RValSeq vs ⟩ l – S k ↓
 | cool_try_err vl1 e2 e3 class reason details xs l k:
   (* in Core Erlang exceptions always have 3 parts *)
-  | xs, RExp e3.[ list_subst [exclass_to_value class; reason; details] idsubst ] | l – k ↓
+  ⟨ xs, RExp e3.[ list_subst [exclass_to_value class; reason; details] idsubst ] ⟩ l – k ↓
 ->
-  | (FTry vl1 e2 3 e3)::xs, RExc (class, reason, details) | l – S k ↓
+  ⟨ (FTry vl1 e2 3 e3)::xs, RExc (class, reason, details) ⟩ l – S k ↓
 (**  Heating *)
 | heat_try e1 vl1 e2 vl2 e3 xs l k:
-  | (FTry vl1 e2 vl2 e3)::xs, RExp e1 | l – k ↓ 
+  ⟨ (FTry vl1 e2 vl2 e3)::xs, RExp e1 ⟩ l – k ↓ 
 ->
-  | xs, ETry e1 vl1 e2 vl2 e3 | l – S k ↓
+  ⟨ xs, ETry e1 vl1 e2 vl2 e3 ⟩ l – S k ↓
   
 (** Exceptions *)
 (** Propogation *)
 | prop_exc F exc xs l k:
   isPropagatable F = true ->
-  | xs, RExc exc | l – k ↓ 
+  ⟨ xs, RExc exc ⟩ l – k ↓ 
 ->
-  | F::xs, RExc exc | l – S k ↓
+  ⟨ F::xs, RExc exc ⟩ l – S k ↓
   (* TODO: details could be appended here to the stack trace *)
 
 (** Ends *)
 | term_fin v :
-  is_result v -> | [] , v | [] – 0 ↓ 
-where "| fs , e | l – k ↓" := (terminates_in_k fs e l k).
+  is_result v -> ⟨ [] , v ⟩ [] – 0 ↓ 
+where "⟨ fs , e ⟩ l – k ↓" := (terminates_in_k fs e l k).
 
 Definition terminates (fs : FrameStack) (e : Redex) (l : list SideEffect) :=
-  exists n, | fs, e | l – n ↓.
-Notation "| fs , e |ₗ l ↓" := (terminates fs e l) (at level 80).
+  exists n, ⟨ fs, e ⟩ l – n ↓.
+Notation "⟨ fs , e ⟩ₗ l ↓" := (terminates fs e l) (at level 0).
 
 
 Ltac inv_term_labeled :=
   match goal with
-  | [H : | _, _ | _ – _ ↓ |- _] => inv H
+  | [H : ⟨ _, _ ⟩ _ – _ ↓ |- _] => inv H
   end.
 Ltac deriv_labeled :=
   match goal with
   | [H : ?i < length _ |- _] => simpl in *; inv H; auto; try lia
   | [H : ?i <= length _ |- _] => simpl in *; inv H;  auto; try lia
-  | [H : | _, _ |ₗ _ ↓ |- _] => inv H; try inv_result
-  | [H : | _ :: _, RValSeq _ |ₗ _ ↓ |- _] => inv H; try inv_result
-  | [H : | _ :: _, RExc _ |ₗ _ ↓ |- _] => inv H; try inv_result
-  | [H : | _, RExp (EExp _) |ₗ _ ↓ |- _] => inv H; try inv_result
-  | [H : | _, RExp (VVal _) |ₗ _ ↓ |- _] => inv H; try inv_result
-  | [H : | _, RBox |ₗ _ ↓ |- _] => inv H; try inv_result
+  | [H : ⟨ _, _ ⟩ₗ _ ↓ |- _] => inv H; try inv_result
+  | [H : ⟨ _ :: _, RValSeq _ ⟩ₗ _ ↓ |- _] => inv H; try inv_result
+  | [H : ⟨ _ :: _, RExc _ ⟩ₗ _ ↓ |- _] => inv H; try inv_result
+  | [H : ⟨ _, RExp (EExp _) ⟩ₗ _ ↓ |- _] => inv H; try inv_result
+  | [H : ⟨ _, RExp (VVal _) ⟩ₗ _ ↓ |- _] => inv H; try inv_result
+  | [H : ⟨ _, RBox ⟩ₗ _ ↓ |- _] => inv H; try inv_result
   end.
 
 Tactic Notation "change" "labeled" "clock" "to" constr(num) :=
   match goal with
-  | |- | _, _ | _ – ?k ↓ => replace k with num by lia
+  | |- ⟨ _, _ ⟩ _ – ?k ↓ => replace k with num by lia
   end.
 
 Theorem inf_diverges :
-  forall n Fs l, ~|Fs, inf| l – n↓.
+  forall n Fs l, ~⟨Fs, inf⟩ l – n↓.
 Proof.
   intros. intro. induction n using Wf_nat.lt_wf_ind.
   inv H. 2: inv H1.
@@ -305,8 +302,8 @@ From CoreErlang.FrameStack Require Export
 
 Lemma labeled_2_unlabeled_termination_equiv :
  forall fs e l n ,
-  | fs, e | l – n ↓ ->
-  | fs, e | n ↓.
+  ⟨ fs, e ⟩ l – n ↓ ->
+  ⟨ fs, e ⟩ n ↓.
 Proof.
   intros fs e l n H.
   induction H; econstructor; eassumption.
@@ -314,8 +311,8 @@ Qed.
 
 Lemma unlabeled_2_labeled_termination_equiv :
  forall fs e n ,
-  | fs, e | n ↓ ->
-  exists l, | fs, e | l – n ↓.
+  ⟨ fs, e ⟩ n ↓ ->
+  exists l, ⟨ fs, e ⟩ l – n ↓.
 Proof.
   intros fs e n H.
   induction H.
