src/FrameStack/Termination.v
@@ -13,165 +13,162 @@ Definition terminates_in_k_sem (fs : FrameStack) (e : Redex) (k : nat)
   : Prop :=
   exists (res : Redex), is_result res /\ ⟨fs, e⟩ -[k]-> ⟨[], res⟩.
 
-
 (** A more practical way to define termination in k steps *)
-Set Warnings "-closed-notation-not-level-0".
 (* The following notation does not work with level 0 *)
-Reserved Notation "| fs , e | k ↓" (at level 80).
-Set Warnings "+closed-notation-not-level-0".
+Reserved Notation "⟨ fs , e ⟩ k ↓" (at level 0).
 Inductive terminates_in_k : FrameStack -> Redex -> nat -> Prop :=
 
 (** Cooling: single value *)
 | cool_value v xs k :
-  | xs, RValSeq [v] | k ↓
+  ⟨ xs, RValSeq [v] ⟩ k ↓
 ->
-  | xs, ˝v | S k ↓
+  ⟨ xs, ˝v ⟩ S k ↓
 
 (************************************************)
 (* heating should be separate for all complex expressions (to be
    syntax-driven).
    Only the intermediate and last steps can be extracted: *)
 | step_params xs ident (el : list Exp) (vl : list Val) (v : Val) (e : Exp) k:
-  | FParams ident (vl ++ [v]) el :: xs, e | k ↓
+  ⟨ FParams ident (vl ++ [v]) el :: xs, e ⟩ k ↓
 ->
-  | FParams ident vl (e :: el) :: xs, RValSeq [v] | S k ↓
+  ⟨ FParams ident vl (e :: el) :: xs, RValSeq [v] ⟩ S k ↓
 
 (* technical rule to avoid duplication for 0 subexpressions : *)
 | step_params_0 xs ident e (el : list Exp) vl k:
   ident <> IMap ->
-  |FParams ident vl el :: xs, RExp e| k ↓
+  ⟨FParams ident vl el :: xs, RExp e⟩ k ↓
 ->
-  |FParams ident vl (e::el) ::xs, RBox| S k ↓
+  ⟨FParams ident vl (e::el) ::xs, RBox⟩ S k ↓
 
 (* 0 subexpression in complex expressions: *)
 | cool_params_0 xs ident (vl : list Val) (res : Redex) (l: option SideEffect) k: 
   ident <> IMap ->
   Some (res, l) = create_result ident vl -> (* TODO side effects *)
-  |xs, res| k ↓
+  ⟨xs, res⟩ k ↓
 ->
-  |FParams ident vl [] ::xs, RBox| S k ↓
+  ⟨FParams ident vl [] ::xs, RBox⟩ S k ↓
 
 | cool_params xs ident (vl : list Val) (v : Val) (res : Redex) (l : option SideEffect) k:
   Some (res, l) = create_result ident (vl ++ [v]) -> (* TODO side effects *)
-  |xs, res| k ↓
+  ⟨xs, res⟩ k ↓
 ->
-  |FParams ident vl [] :: xs, RValSeq [v]| S k ↓
+  ⟨FParams ident vl [] :: xs, RValSeq [v]⟩ S k ↓
 
 (************************************************)
 (* Heating constructs with list subexpressions: *)
 | heat_values (el : list Exp) (xs : list Frame) k:
-  | (FParams IValues [] el)::xs, RBox | k ↓
+  ⟨ (FParams IValues [] el)::xs, RBox ⟩ k ↓
 ->
-  | xs, EValues el | S k ↓
+  ⟨ xs, EValues el ⟩ S k ↓
 
 | heat_tuple (el : list Exp) (xs : list Frame) k:
-  | (FParams ITuple [] el)::xs, RBox | k ↓ 
+  ⟨ (FParams ITuple [] el)::xs, RBox ⟩ k ↓ 
 ->
-  | xs, ETuple el | S k ↓
+  ⟨ xs, ETuple el ⟩ S k ↓
 
 (* This is handled separately, to satisfy the invariant in FCLOSED for maps *)
 | heat_map_0 (xs : list Frame) k:
-  | xs, RValSeq [VMap []] | k ↓ 
+  ⟨ xs, RValSeq [VMap []] ⟩ k ↓ 
 ->
-  | xs, EMap [] | S k ↓
+  ⟨ xs, EMap [] ⟩ S k ↓
 
 | heat_map (e1 e2 : Exp) (el : list (Exp * Exp)) (xs : list Frame) k:
-  | (FParams IMap [] (e2 :: flatten_list el))::xs, e1 | k ↓ 
+  ⟨ (FParams IMap [] (e2 :: flatten_list el))::xs, e1 ⟩ k ↓ 
 ->
-  | xs, EMap ((e1, e2) :: el) | S k ↓
+  ⟨ xs, EMap ((e1, e2) :: el) ⟩ S k ↓
 
 | heat_call_mod (el : list Exp) (xs : list Frame) (m f : Exp) k :
-  | FCallMod f el :: xs, m | k ↓
+  ⟨ FCallMod f el :: xs, m ⟩ k ↓
 ->
-  | xs, ECall m f el | S k ↓
+  ⟨ xs, ECall m f el ⟩ S k ↓
 
 | heat_call_fun (el : list Exp) (xs : list Frame) (v : Val) (f : Exp) k :
-  | FCallFun v el :: xs, f | k ↓
+  ⟨ FCallFun v el :: xs, f ⟩ k ↓
 ->
-  | FCallMod f el :: xs, RValSeq [v] | S k ↓
+  ⟨ FCallMod f el :: xs, RValSeq [v] ⟩ S k ↓
 
 | heat_call_params (el : list Exp) (xs : list Frame) (m f : Val) k:
-  | (FParams (ICall m f) [] el)::xs, RBox | k ↓
+  ⟨ (FParams (ICall m f) [] el)::xs, RBox ⟩ k ↓
 ->
-  | FCallFun m el :: xs, RValSeq [f] | S k ↓
+  ⟨ FCallFun m el :: xs, RValSeq [f]⟩ S k ↓
 
 | heat_primop (el : list Exp) (xs : list Frame) f k:
-  | (FParams (IPrimOp f) [] el)::xs, RBox | k ↓ 
+  ⟨ (FParams (IPrimOp f) [] el)::xs, RBox ⟩ k ↓ 
 ->
-  | xs, EPrimOp f el | S k ↓
+  ⟨ xs, EPrimOp f el ⟩ S k ↓
 
 | heat_app2 (el : list Exp) (xs : list Frame) (v : Val) k:
-  | (FParams (IApp v) [] el)::xs, RBox | k ↓ 
+  ⟨ (FParams (IApp v) [] el)::xs, RBox ⟩ k ↓ 
 ->
-  | FApp1 el :: xs, RValSeq [v] | S k ↓
+  ⟨ FApp1 el :: xs, RValSeq [v] ⟩ S k ↓
 
 (************************************************)
 (**  App *)
 | heat_app xs e l k:
-  |FApp1 l :: xs, RExp e|  k ↓ 
+  ⟨FApp1 l :: xs, RExp e⟩  k ↓ 
 ->
-  |xs, EApp e l| S k ↓
+  ⟨xs, EApp e l⟩ S k ↓
 (**  List *)
 (**  Cooling *)
 
 | cool_cons_1 (hd : Exp) (tl : Val) xs k :
-  | (FCons2 tl)::xs, RExp hd | k ↓ 
+  ⟨ (FCons2 tl)::xs, RExp hd ⟩ k ↓ 
 ->
-  | (FCons1 hd)::xs, RValSeq [tl] | S k ↓
+  ⟨ (FCons1 hd)::xs, RValSeq [tl] ⟩ S k ↓
 
 | cool_cons_2 (hd tl : Val) xs k:
-  | xs, RValSeq [VCons hd tl] | k ↓ 
+  ⟨ xs, RValSeq [VCons hd tl] ⟩ k ↓ 
 ->
-  | (FCons2 tl)::xs, RValSeq [hd] | S k ↓
+  ⟨ (FCons2 tl)::xs, RValSeq [hd] ⟩ S k ↓
 
 (**  Heating *)
 | heat_cons (hd tl : Exp) xs k:
-  | (FCons1 hd)::xs, RExp tl | k ↓ 
+  ⟨ (FCons1 hd)::xs, RExp tl ⟩ k ↓ 
 ->
-  | xs, ECons hd tl | S k ↓
+  ⟨ xs, ECons hd tl ⟩ S k ↓
 
 (**  Let *)
 (**  Cooling *)
 | cool_let l e2 vs xs k:
   length vs = l ->
-  | xs, RExp (e2.[ list_subst vs idsubst ]) | k ↓ 
+  ⟨ xs, RExp (e2.[ list_subst vs idsubst ]) ⟩ k ↓ 
 ->
-  | (FLet l e2)::xs, RValSeq vs | S k ↓
+  ⟨ (FLet l e2)::xs, RValSeq vs ⟩ S k ↓
 
 (**  Heating *)
 | heat_let l e1 e2 xs k:
-  | (FLet l e2)::xs, RExp e1 | k ↓ 
+  ⟨ (FLet l e2)::xs, RExp e1 ⟩ k ↓ 
 ->
-  | xs, ELet l e1 e2 | S k ↓
+  ⟨ xs, ELet l e1 e2 ⟩ S k ↓
 
 (**  Seq *)
 (**  Cooling *)
 | cool_seq e2 v xs k:
-  | xs, RExp e2 | k ↓ 
+  ⟨ xs, RExp e2 ⟩ k ↓ 
 ->
-  | (FSeq e2)::xs, RValSeq [v] | S k ↓
+  ⟨ (FSeq e2)::xs, RValSeq [v] ⟩ S k ↓
 (**  Heating *)
 | heat_seq e1 e2 xs k:
-  | (FSeq e2)::xs, RExp e1 | k ↓ 
+  ⟨ (FSeq e2)::xs, RExp e1 ⟩ k ↓ 
 ->
-  | xs, ESeq e1 e2 | S k ↓
+  ⟨ xs, ESeq e1 e2 ⟩ S k ↓
 
 
 (**  Fun *)
 (**  Cooling *)
 | cool_fun e vl xs k:
-  | xs, RValSeq [ VClos [] 0 vl e ] | k ↓ 
+  ⟨ xs, RValSeq [ VClos [] 0 vl e ] ⟩ k ↓ 
 ->
-  | xs, EFun vl e | S k ↓
+  ⟨ xs, EFun vl e ⟩ S k ↓
   (* TODO : id <> 0 usually *)
 
 
 (**  Case *)
 (**  Heating *)
 | heat_case e l xs k:
-  | (FCase1 l)::xs, RExp e | k ↓ 
+  ⟨ (FCase1 l)::xs, RExp e ⟩ k ↓ 
 ->
-  | xs, ECase e l | S k ↓
+  ⟨ xs, ECase e l ⟩ S k ↓
 
 (**  Cooling *)
 (* reduction started or it is already ongoing, the first pattern matched,
@@ -179,36 +176,36 @@ Inductive terminates_in_k : FrameStack -> Redex -> nat -> Prop :=
    matching is stored in the frame) *)
 | step_case_match lp e1 e2 l vs vs' xs k:
   match_pattern_list lp vs = Some vs' ->
-  | (FCase2 vs e2.[list_subst vs' idsubst] l)::xs, RExp (e1.[list_subst vs' idsubst]) | k ↓
+  ⟨ (FCase2 vs e2.[list_subst vs' idsubst] l)::xs, RExp (e1.[list_subst vs' idsubst]) ⟩ k ↓
 ->
-  | (FCase1 ((lp,e1,e2)::l))::xs, RValSeq vs | S k ↓
+  ⟨ (FCase1 ((lp,e1,e2)::l))::xs, RValSeq vs ⟩ S k ↓
 (* reduction started or it is already ongoing, the first pattern doesn't 
    match, so we check the next pattern *)
 | step_case_not_match lp e1 e2 l vs xs k:
   match_pattern_list lp vs = None ->
-  | (FCase1 l)::xs, RValSeq vs | k ↓ 
+  ⟨ (FCase1 l)::xs, RValSeq vs ⟩ k ↓ 
 ->
-  | (FCase1 ((lp,e1,e2)::l))::xs, RValSeq vs | S k ↓
+  ⟨ (FCase1 ((lp,e1,e2)::l))::xs, RValSeq vs ⟩ S k ↓
 
 (* reduction is ongoing, the pattern matched, and the guard is true, thus 
    the reduction continues inside the given clause *)
 | step_case_true vs e' l xs k:
-  | xs, RExp e' | k ↓ 
+  ⟨ xs, RExp e' ⟩ k ↓ 
 ->
-  | (FCase2 vs e' l)::xs, RValSeq [ VLit (Atom "true") ] | S k ↓
+  ⟨ (FCase2 vs e' l)::xs, RValSeq [ VLit (Atom "true") ] ⟩ S k ↓
 
 (* reduction is ongoing, the pattern matched, and the guard is false, thus
    we check the next pattern. *)
 | step_case_false vs e' l xs k:
-  | (FCase1 l)::xs, RValSeq vs | k ↓ 
+  ⟨ (FCase1 l)::xs, RValSeq vs ⟩ k ↓ 
 ->
-  | (FCase2 vs e' l)::xs, RValSeq [ VLit (Atom "false") ] | S k ↓
+  ⟨ (FCase2 vs e' l)::xs, RValSeq [ VLit (Atom "false") ] ⟩ S k ↓
 
 (** Exceptions *)
 | cool_case_empty vs xs k:
-  | xs, RExc if_clause | k ↓ 
+  ⟨ xs, RExc if_clause ⟩ k ↓ 
 ->
-  | (FCase1 [])::xs, RValSeq vs | S k ↓
+  ⟨ (FCase1 [])::xs, RValSeq vs ⟩ S k ↓
 
 (**  LetRec *)
 (**  Cooling *)
@@ -216,71 +213,71 @@ Inductive terminates_in_k : FrameStack -> Redex -> nat -> Prop :=
 | heat_letrec l e lc xs k:
   convert_to_closlist (map (fun '(x,y) => (0,x,y)) l) = lc ->
   (* TODO: for now the funids are 0 coded in *)
-  | xs, RExp e.[list_subst lc idsubst] | k ↓ 
+  ⟨ xs, RExp e.[list_subst lc idsubst] ⟩ k ↓ 
 ->
-  | xs, ELetRec l e | S k ↓
+  ⟨ xs, ELetRec l e ⟩ S k ↓
 
 
 (**  Try *)
 (**  Cooling *)
 | cool_try_ok vl1 e2 vl2 e3 vs xs k:
   vl1 = length vs ->
-  | xs, RExp e2.[ list_subst vs idsubst ] | k ↓ 
+  ⟨ xs, RExp e2.[ list_subst vs idsubst ] ⟩ k ↓ 
 ->
-  | (FTry vl1 e2 vl2 e3)::xs, RValSeq vs | S k ↓
+  ⟨ (FTry vl1 e2 vl2 e3)::xs, RValSeq vs ⟩ S k ↓
 | cool_try_err vl1 e2 e3 class reason details xs k:
   (* in Core Erlang exceptions always have 3 parts *)
-  | xs, RExp e3.[ list_subst [exclass_to_value class; reason; details] idsubst ] | k ↓
+  ⟨ xs, RExp e3.[ list_subst [exclass_to_value class; reason; details] idsubst ] ⟩ k ↓
 ->
-  | (FTry vl1 e2 3 e3)::xs, RExc (class, reason, details) | S k ↓
+  ⟨ (FTry vl1 e2 3 e3)::xs, RExc (class, reason, details) ⟩ S k ↓
 (**  Heating *)
 | heat_try e1 vl1 e2 vl2 e3 xs k:
-  | (FTry vl1 e2 vl2 e3)::xs, RExp e1 | k ↓ 
+  ⟨ (FTry vl1 e2 vl2 e3)::xs, RExp e1 ⟩ k ↓ 
 ->
-  | xs, ETry e1 vl1 e2 vl2 e3 | S k ↓
+  ⟨ xs, ETry e1 vl1 e2 vl2 e3 ⟩ S k ↓
   
 (** Exceptions *)
 (** Propogation *)
 | prop_exc F exc xs k:
   isPropagatable F = true ->
-  | xs, RExc exc | k ↓ 
+  ⟨ xs, RExc exc ⟩ k ↓ 
 ->
-  | F::xs, RExc exc | S k ↓
+  ⟨ F::xs, RExc exc ⟩ S k ↓
   (* TODO: details could be appended here to the stack trace *)
 
 (** Ends *)
 | term_fin res :
-  is_result res -> | [] , res | 0 ↓ 
-where "| fs , e | k ↓" := (terminates_in_k fs e k).
+  is_result res -> ⟨ [] , res ⟩ 0 ↓ 
+where "⟨ fs , e ⟩ k ↓" := (terminates_in_k fs e k).
 
 Definition terminates (fs : FrameStack) (e : Redex) :=
-  exists n, | fs, e | n ↓.
-Notation "| fs , e | ↓" := (terminates fs e) (at level 80).
+  exists n, ⟨ fs, e ⟩ n ↓.
+Notation "⟨ fs , e ⟩ ↓" := (terminates fs e) (at level 0).
 
 
 Ltac inv_term :=
   match goal with
-  | [H : | _, _ | _ ↓ |- _] => inv H
+  | [H : ⟨ _, _ ⟩ _ ↓ |- _] => inv H
   end.
 Ltac deriv :=
   match goal with
   | [H : ?i < length _ |- _] => simpl in *; inv H; auto; try lia
   | [H : ?i <= length _ |- _] => simpl in *; inv H;  auto; try lia
-  | [H : | _, _ | ↓ |- _] => inv H; try inv_result
-  | [H : | _ :: _, RValSeq _ | _ ↓ |- _] => inv H; try inv_result
-  | [H : | _ :: _, RExc _ | _ ↓ |- _] => inv H; try inv_result
-  | [H : | _, RExp (EExp _) | _ ↓ |- _] => inv H; try inv_result
-  | [H : | _, RExp (VVal _) | _ ↓ |- _] => inv H; try inv_result
-  | [H : | _, RBox | _ ↓ |- _] => inv H; try inv_result
+  | [H : ⟨ _, _ ⟩ ↓ |- _] => inv H; try inv_result
+  | [H : ⟨ _ :: _, RValSeq _ ⟩ _ ↓ |- _] => inv H; try inv_result
+  | [H : ⟨ _ :: _, RExc _ ⟩ _ ↓ |- _] => inv H; try inv_result
+  | [H : ⟨ _, RExp (EExp _) ⟩ _ ↓ |- _] => inv H; try inv_result
+  | [H : ⟨ _, RExp (VVal _) ⟩ _ ↓ |- _] => inv H; try inv_result
+  | [H : ⟨ _, RBox ⟩ _ ↓ |- _] => inv H; try inv_result
   end.
 
 Tactic Notation "change" "clock" "to" constr(num) :=
   match goal with
-  | |- | _, _ | ?k ↓ => replace k with num by lia
+  | |- ⟨ _, _ ⟩ ?k ↓ => replace k with num by lia
   end.
 
 Theorem inf_diverges :
-  forall n Fs, ~|Fs, inf| n↓.
+  forall n Fs, ~⟨Fs, inf⟩ n↓.
 Proof.
   intros. intro. induction n using Wf_nat.lt_wf_ind.
   deriv. simpl in *. deriv. do 3 deriv.
