src/Concurrent/NodeSemantics.v
@@ -558,11 +558,11 @@ Qed.
 Definition renamePIDPool (p p' : PID) (Π : ProcessPool) : ProcessPool :=
   kmap (renamePIDPID_sym p p') (renamePIDProc p p' <$> Π).
 
-Notation "e .[ x ⇔ y ]ₚₚ" := (renamePIDPool x y e) (at level 2, left associativity).
+Notation "e .[ x ⇔ y ]ₚₚ" := (renamePIDPool x y e) (at level 1, left associativity).
 
 (* ONLY keys are symmetrically replaced  *)
 Definition renamePIDEther (p p' : PID) (eth : Ether) : Ether :=
   kmap (prod_map (renamePIDPID_sym p p') (renamePIDPID_sym p p'))
     ((map (renamePIDSignal p p')) <$> eth).
 
-Notation "e .[ x ⇔ y ]ₑ" := (renamePIDEther x y e) (at level 2, left associativity).
+Notation "e .[ x ⇔ y ]ₑ" := (renamePIDEther x y e) (at level 1, left associativity).
